ironfleet/src/Dafny/Distributed/Protocol/RSL/FailureProof/Phase1/GenericLemmas.i.dfy
@@ -1,0 +1,129 @@
+include "Phase1Proof.i.dfy"
+
+module RslPhase1Proof_Generic {
+import opened RslPhase1Proof_i
+
+/* There can be no 1a messages sent in a
+* non-LReplicaNextSpontaneousMaybeEnterNewViewAndSend1a step  */
+lemma lemma_No1aSentInNon1aStep(ts:TimestampedRslState, ts':TimestampedRslState, op:OperationNumber, idx:int, tios:seq<TimestampedLIoOp<NodeIdentity, RslMessage>>) 
+    requires CommonAssumptions(ts) && CommonAssumptions(ts')
+    requires P1Assumption(ts, op)
+    requires TimestampedRslNext(ts, ts')
+    requires !TimestampedRslNextEnvironment(ts, ts')
+    requires TimestampedRslNextOneReplica(ts, ts', idx, tios)
+    requires Phase1Invariant(ts, op)
+    requires idx != 0
+    requires ts.t_replicas[idx].v.nextActionIndex != 1
+    ensures forall p | p in ts'.t_environment.sentPackets && p.msg.v.RslMessage_1a? :: p in ts.t_environment.sentPackets
+    ensures forall p | p in ts'.undeliveredPackets && p.msg.v.RslMessage_1a? :: p in ts.undeliveredPackets
+{
+    var ls, ls' := ts.t_replicas[idx], ts'.t_replicas[idx];
+    var nextActionIndex := ls.v.nextActionIndex;
+
+    forall p | p in ts'.t_environment.sentPackets && p.msg.v.RslMessage_1a?
+    ensures p in ts.t_environment.sentPackets {
+        if p !in ts.t_environment.sentPackets {
+            if nextActionIndex == 2 {
+                assert false;
+            } else {
+                forall io | io in tios && io.LIoOpSend?
+                ensures !io.s.msg.v.RslMessage_1a? {}
+                assert false;
+            }
+        }
+    }
+    lemma_No1aSentInNon1aStep_Undelivered(ts, ts', op, idx, tios);
+}
+
+lemma lemma_No1aSentInNon1aStep_Undelivered(ts:TimestampedRslState, ts':TimestampedRslState, op:OperationNumber, idx:int, tios:seq<TimestampedLIoOp<NodeIdentity, RslMessage>>) 
+    requires CommonAssumptions(ts) && CommonAssumptions(ts')
+    requires P1Assumption(ts, op)
+    requires TimestampedRslNext(ts, ts')
+    requires !TimestampedRslNextEnvironment(ts, ts')
+    requires TimestampedRslNextOneReplica(ts, ts', idx, tios)
+    requires Phase1Invariant(ts, op)
+    requires idx != 0
+    requires ts.t_replicas[idx].v.nextActionIndex != 1
+    ensures forall p | p in ts'.undeliveredPackets && p.msg.v.RslMessage_1a? :: p in ts.undeliveredPackets
+{
+    var ls, ls' := ts.t_replicas[idx], ts'.t_replicas[idx];
+    var nextActionIndex := ls.v.nextActionIndex;
+
+    forall p | p in ts'.undeliveredPackets && p.msg.v.RslMessage_1a?
+    ensures p in ts.undeliveredPackets {
+        if p !in ts.undeliveredPackets {
+            if nextActionIndex == 2 {
+                assert false;
+            } else {
+                forall io | io in tios && io.LIoOpSend?
+                ensures !io.s.msg.v.RslMessage_1a? {}
+                assert false;
+            }
+        }
+    }
+}
+
+
+/* Non-leader replicas do not send 1a's */
+lemma lemma_NonLeaderDoesNotSend1a(ts:TimestampedRslState, ts':TimestampedRslState, op:OperationNumber, idx:int, tios:seq<TimestampedLIoOp<NodeIdentity, RslMessage>>) 
+    requires CommonAssumptions(ts) && CommonAssumptions(ts')
+    requires P1Assumption(ts, op)
+    requires TimestampedRslNext(ts, ts')
+    requires !TimestampedRslNextEnvironment(ts, ts')
+    requires TimestampedRslNextOneReplica(ts, ts', idx, tios)
+    requires Phase1Invariant(ts, op)
+    requires idx != 0
+    requires idx != 1
+    ensures forall p | p in ts'.t_environment.sentPackets && p.msg.v.RslMessage_1a? :: p in ts.t_environment.sentPackets
+    ensures forall p | p in ts'.undeliveredPackets && p.msg.v.RslMessage_1a? :: p in ts.undeliveredPackets
+{
+    var ls, ls' := ts.t_replicas[idx], ts'.t_replicas[idx];
+    var nextActionIndex := ls.v.nextActionIndex;
+    forall p | p in ts'.t_environment.sentPackets && p.msg.v.RslMessage_1a?
+    ensures p in ts.t_environment.sentPackets {
+        if p !in ts.t_environment.sentPackets {
+            if nextActionIndex == 1 {
+                assert ReplicasDistinct(ts'.constants.config.replica_ids, ls.v.replica.proposer.election_state.current_view.proposer_id, idx);
+                assert ls.v.replica.proposer.election_state.current_view.proposer_id != ls.v.replica.proposer.constants.my_index;
+                assert forall io | io in tios && io.LIoOpSend? :: !io.s.msg.v.RslMessage_1a?;
+                assert false;
+            } else {
+                lemma_No1aSentInNon1aStep(ts, ts', op, idx, tios);
+                assert false;
+            }
+        }
+    }
+    lemma_NonLeaderDoesNotSend1a_Undelivered(ts, ts', op, idx, tios);
+}
+
+/* Non-leader replicas do not send 1a's */
+lemma lemma_NonLeaderDoesNotSend1a_Undelivered(ts:TimestampedRslState, ts':TimestampedRslState, op:OperationNumber, idx:int, tios:seq<TimestampedLIoOp<NodeIdentity, RslMessage>>) 
+    requires CommonAssumptions(ts) && CommonAssumptions(ts')
+    requires P1Assumption(ts, op)
+    requires TimestampedRslNext(ts, ts')
+    requires !TimestampedRslNextEnvironment(ts, ts')
+    requires TimestampedRslNextOneReplica(ts, ts', idx, tios)
+    requires Phase1Invariant(ts, op)
+    requires idx != 0
+    requires idx != 1
+    ensures forall p | p in ts'.undeliveredPackets && p.msg.v.RslMessage_1a? :: p in ts.undeliveredPackets
+{
+    var ls, ls' := ts.t_replicas[idx], ts'.t_replicas[idx];
+    var nextActionIndex := ls.v.nextActionIndex;
+    forall p | p in ts'.undeliveredPackets && p.msg.v.RslMessage_1a?
+    ensures p in ts.undeliveredPackets {
+        if p !in ts.undeliveredPackets {
+            if nextActionIndex == 1 {
+                assert ReplicasDistinct(ts'.constants.config.replica_ids, ls.v.replica.proposer.election_state.current_view.proposer_id, idx);
+                assert ls.v.replica.proposer.election_state.current_view.proposer_id != ls.v.replica.proposer.constants.my_index;
+                assert forall io | io in tios && io.LIoOpSend? :: !io.s.msg.v.RslMessage_1a?;
+                assert false;
+            } else {
+                lemma_No1aSentInNon1aStep(ts, ts', op, idx, tios);
+                assert false;
+            }
+        }
+    }
+}
+
+}
