ironfleet/src/Dafny/Distributed/Protocol/RSL/FailureProof/Phase1/Phase1Proof_helper1.i.dfy
@@ -1,9 +1,9 @@
 include "Phase1Proof.i.dfy"
-// include "GenericLemmas.i.dfy"
+include "GenericLemmas.i.dfy"
 
 module RslPhase1Proof_Helper1 {
 import opened RslPhase1Proof_i
-// import opened RslPhase1Proof_Generic
+import opened RslPhase1Proof_Generic
 
 
 lemma PacketsBallotInvariant_ReceiveStep(ts:TimestampedRslState, ts':TimestampedRslState, opn:OperationNumber, idx:int, tios:seq<TimestampedLIoOp<NodeIdentity, RslMessage>>) 
@@ -36,6 +36,95 @@ lemma PacketsBallotInvariant_NoReceiveStep(ts:TimestampedRslState, ts':Timestamp
     forall pkt | pkt in ts'.undeliveredPackets 
     ensures ExistingPacketsBallot(pkt)
     {}
+}
+
+
+/* Proof that a Phase1 state transitions to a Phase1 state when nextAction != 2 */
+lemma Phase1_to_Phase1(ts:TimestampedRslState, ts':TimestampedRslState, opn:OperationNumber, idx:int, tios:seq<TimestampedLIoOp<NodeIdentity, RslMessage>>) 
+    requires CommonAssumptions(ts) && CommonAssumptions(ts')
+    requires P1Assumption(ts, opn)
+    requires InPhase1(ts') ==> P1Assumption(ts', opn)
+    requires TimestampedRslNext(ts, ts')
+    requires Phase1Invariant(ts, opn)
+    requires TimestampedRslNextOneReplica(ts, ts', idx, tios);
+    requires ts.t_replicas[idx].v.nextActionIndex != 2
+    requires idx != 0
+    ensures InPhase1(ts')
+    ensures PerfInvariant(ts', opn)
+{
+    assert InPhase1(ts');
+    Phase1_to_Phase1_LeaderTimeBound(ts, ts', opn, idx, tios);
+    Phase1_to_Phase1_1aTimeboud(ts, ts', opn, idx, tios);
+}
+
+lemma Phase1_to_Phase1_1aTimeboud(ts:TimestampedRslState, ts':TimestampedRslState, opn:OperationNumber, idx:int, tios:seq<TimestampedLIoOp<NodeIdentity, RslMessage>>) 
+    requires CommonAssumptions(ts) && CommonAssumptions(ts')
+    requires P1Assumption(ts, opn)
+    requires P1Assumption(ts', opn)
+    requires TimestampedRslNext(ts, ts')
+    requires Phase1Invariant(ts, opn)
+    requires TimestampedRslNextOneReplica(ts, ts', idx, tios);
+    requires ts.t_replicas[idx].v.nextActionIndex != 2
+    requires idx != 0
+    ensures forall pkt | pkt in ts'.undeliveredPackets && IsNew1aPacket(pkt)
+        :: TimeLe(pkt.msg.ts, TimeBound1aDeliveryPost())
+{   
+    var ls, ls' := ts.t_replicas[idx], ts'.t_replicas[idx];
+    var nextActionIndex := ls.v.nextActionIndex;
+
+    if idx == 1 {
+        if nextActionIndex == 1 {
+            assert !BalLt(ls.v.replica.proposer.max_ballot_i_sent_1a, ls.v.replica.proposer.election_state.current_view);
+            forall io | io in tios 
+            ensures !io.LIoOpSend? {}
+        } else {
+            lemma_No1aSentInNon1aStep(ts, ts', opn, idx, tios);
+        }
+    } else {
+        lemma_NonLeaderDoesNotSend1a(ts, ts', opn, idx, tios);
+    }
+}
+
+
+lemma Phase1_to_Phase1_LeaderTimeBound(ts:TimestampedRslState, ts':TimestampedRslState, opn:OperationNumber, idx:int, tios:seq<TimestampedLIoOp<NodeIdentity, RslMessage>>) 
+    requires CommonAssumptions(ts) && CommonAssumptions(ts')
+    requires P1Assumption(ts, opn)
+    requires P1Assumption(ts', opn)
+    requires TimestampedRslNext(ts, ts')
+    requires Phase1Invariant(ts, opn)
+    requires TimestampedRslNextOneReplica(ts, ts', idx, tios);
+    requires ts.t_replicas[idx].v.nextActionIndex != 2
+    requires idx != 0
+    ensures TimeLe(ts'.t_replicas[1].ts, TimeBoundPhase1LeaderPost(ts'.t_replicas[1].v.nextActionIndex))
+{  
+    if idx != 1 {
+        assert ts'.t_replicas[1].ts == ts.t_replicas[1].ts;
+        return;
+    }
+    var ls, ls' := ts.t_replicas[1], ts'.t_replicas[1];
+    var nextActionIndex, nextActionIndex' := ls.v.nextActionIndex, ls'.v.nextActionIndex;
+
+    if nextActionIndex == 0 {
+        var pkt := tios[0].r;
+        assert ts.t_environment.nextStep.nodeStep == RslStep(0);
+        if pkt.msg.v.RslMessage_1a? {
+            assert IsNew1aPacket(pkt);
+            assert TimeLe(pkt.msg.ts, TimeBound1aDeliveryPost());
+            assert TimeLe(pkt.msg.ts, TimeBound1bDeliveryPost());
+        } else if pkt.msg.v.RslMessage_1b? {
+            assert IsNew1bPacket(pkt);
+            assert TimeLe(pkt.msg.ts, TimeBound1bDeliveryPost());
+        } else {
+            assert false;
+        }
+        assert TimeLe(TimeMax(pkt.msg.ts, ls.ts), pkt.msg.ts + MaxQueueTime);
+        assert TimeLe(ls'.ts, pkt.msg.ts + MaxQueueTime + StepToTimeDelta(RslStep(0)));
+        assert TimeLe(ls'.ts, TimeBound1bDeliveryPost() + MaxQueueTime + TimeActionRange(1));
+        assert TimeLe(ls'.ts, TimeBoundPhase1LeaderPost(nextActionIndex'));
+    } else {
+        var hstep := ts.t_environment.nextStep.nodeStep;
+        assert hstep == RslStep(nextActionIndex);
+    }
 }
 
 }
