ironfleet/src/Dafny/Distributed/Protocol/RSL/FailureProof/Phase1/verify.sh
@@ -1,8 +1,12 @@
 #!/bin/bash -li
 
-# echo ""
-# echo "Verifying GenericLemmas.i.dfy"
-# dafny GenericLemmas.i.dfy | grep -iv "Warning"
+echo ""
+echo "Verifying Phase1Proof.i.dfy"
+dafny Phase1Proof.i.dfy | grep -iv "Warning"
+
+echo ""
+echo "Verifying GenericLemmas.i.dfy"
+dafny GenericLemmas.i.dfy | grep -iv "Warning"
 
 echo ""
 echo "Verifying Phase1Proof_helper0.i.dfy"
@@ -16,9 +20,6 @@ dafny Phase1Proof_helper0.i.dfy | grep -iv "Warning"
 # echo "Verifying Phase2Proof_helper2.i.dfy"
 # dafny Phase2Proof_helper2.i.dfy | grep -iv "Warning"
 
-echo ""
-echo "Verifying Phase1Proof.i.dfy"
-dafny Phase1Proof.i.dfy | grep -iv "Warning"
 
 echo ""
 echo "Verifying Phase1Proof_toplevel.i.dfy"
